compose/SimSymbDrop.v
@@ -739,7 +739,7 @@ Next Obligation.
   inv MLE. inv SIMSKENV.
   assert (SAME: forall b b' delta, Plt b (Genv.genv_next skenv_src) ->
                                    inj sm1 b = Some(b', delta) -> inj sm0 b = Some(b', delta)).
-  { i. erewrite frozen_preserves_src; eauto. i. xomega. }
+  { i. erewrite frozen_preserves_src; eauto. congruence. }
   apply sim_skenv_splittable_spec.
   rr.
   dsplits; eauto; try congruence; ii.
@@ -753,14 +753,42 @@ Next Obligation.
     exfalso.
     inv FROZEN. exploit NEW_IMPLIES_OUTSIDE; eauto. i; des.
     exploit SPLITHINT; try apply SYMBSRC; eauto. i; des. clear_tac.
-    exploit Genv.genv_symb_range; eauto. i. clear - H OUTSIDE_TGT BOUNDTGT. xomega.
+    exploit Genv.genv_symb_range; eauto. i. clear - H OUTSIDE_TGT NBTGT.
+    exploit Plt_Ple_trans; try apply OUTSIDE_TGT. { rewrite <- NBTGT. et. } i. xomega.
   - i. eapply SIMDEFINV; eauto.
     destruct (inj sm0 blk_src) as [[b1 delta1] | ] eqn: J.
     + exploit INCR; eauto. congruence.
     + inv FROZEN. exploit NEW_IMPLIES_OUTSIDE; eauto. i; des.
-      exploit Genv.genv_defs_range; eauto. xomega.
+      exploit Genv.genv_defs_range; eauto. i.
+      exploit Plt_Ple_trans; try apply OUTSIDE_TGT. { rewrite <- NBTGT. et. } i. xomega.
   (* admit "The proof must exist in Unusedglobproof.v. See match_stacks_preserves_globals, match_stacks_incr". *)
 Qed.
+(* Next Obligation. *)
+(*   inv MLE. inv SIMSKENV. *)
+(*   assert (SAME: forall b b' delta, Plt b (Genv.genv_next skenv_src) -> *)
+(*                                    inj sm1 b = Some(b', delta) -> inj sm0 b = Some(b', delta)). *)
+(*   { i. erewrite frozen_preserves_src; eauto. i. xomega. } *)
+(*   apply sim_skenv_splittable_spec. *)
+(*   rr. *)
+(*   dsplits; eauto; try congruence; ii. *)
+(*   - i. eapply SIMSYMB1; eauto. eapply SAME; try eapply Genv.genv_symb_range; eauto. *)
+(*   - i. exploit SIMSYMB2; eauto. i; des. eexists. splits; eauto. *)
+(*   - i. exploit SIMSYMB3; eauto. i; des. eexists. splits; eauto. *)
+(*   - i. exploit SIMDEF; eauto. eapply SAME; try eapply Genv.genv_defs_range; eauto. *)
+(*   - i. eapply DISJ; eauto. eapply SAME; try eapply Genv.genv_symb_range; eauto. *)
+(*     destruct (inj sm0 blk_src1) eqn:T; ss. *)
+(*     { destruct p; ss. exploit INCR; et. i; clarify. } *)
+(*     exfalso. *)
+(*     inv FROZEN. exploit NEW_IMPLIES_OUTSIDE; eauto. i; des. *)
+(*     exploit SPLITHINT; try apply SYMBSRC; eauto. i; des. clear_tac. *)
+(*     exploit Genv.genv_symb_range; eauto. i. clear - H OUTSIDE_TGT BOUNDTGT. xomega. *)
+(*   - i. eapply SIMDEFINV; eauto. *)
+(*     destruct (inj sm0 blk_src) as [[b1 delta1] | ] eqn: J. *)
+(*     + exploit INCR; eauto. congruence. *)
+(*     + inv FROZEN. exploit NEW_IMPLIES_OUTSIDE; eauto. i; des. *)
+(*       exploit Genv.genv_defs_range; eauto. xomega. *)
+(*   (* admit "The proof must exist in Unusedglobproof.v. See match_stacks_preserves_globals, match_stacks_incr". *) *)
+(* Qed. *)
 Next Obligation.
   set (SkEnv.project skenv_link_src sk_src) as skenv_src.
   generalize (SkEnv.project_impl_spec INCLSRC); intro LESRC.
