proof/MatchSimModSemSR.v
@@ -4,6 +4,7 @@ Require Import Simulation.
 Require Import ModSem AsmregsC GlobalenvsC MemoryC ASTC.
 Require Import Skeleton SimModSemSR SimMem SimSymb.
 Require Import Sound Preservation.
+Require Import ModSemProps.
 
 Set Implicit Arguments.
 
@@ -121,7 +122,7 @@ Section MATCHSIMFORWARD.
       (MLE: SimMem.le sm0 sm_arg)
       (* (MWF: SimMem.wf sm_arg) *)
       sm_ret
-      (MLE: SimMem.le (SimMem.lift sm_arg) sm_ret)
+      (MLE: SimMem.lepriv sm_arg sm_ret)
       (MWF: SimMem.wf sm_ret)
       retv_src retv_tgt
       (SIMRET: SimMem.sim_retv retv_src retv_tgt sm_ret)
@@ -133,15 +134,17 @@ Section MATCHSIMFORWARD.
       (HISTORY: match_states_at_helper sm_init idx0 st_src0 st_tgt0 sm0 sm_arg)
 
       (* just helpers *)
-      (MWFAFTR: SimMem.wf (SimMem.unlift sm_arg sm_ret))
-      (MLEAFTR: SimMem.le sm_arg (SimMem.unlift sm_arg sm_ret))
+      (* (MWFAFTR: SimMem.wf (SimMem.unlift sm_arg sm_ret)) *)
+      (* (MLEAFTR: SimMem.le sm_arg (SimMem.unlift sm_arg sm_ret)) *)
     ,
       exists sm_after idx1 st_tgt1,
         (<<AFTERTGT: ms_tgt.(ModSem.after_external) st_tgt0 retv_tgt st_tgt1>>)
         /\
         (<<MATCH: match_states sm_init idx1 st_src1 st_tgt1 sm_after>>)
         /\
-        (<<MLE: SimMem.le (SimMem.unlift sm_arg sm_ret) sm_after>>)
+        (<<MLE: SimMem.lepriv sm_ret sm_after>>)
+        /\
+        (<<MLE: SimMem.le sm0 sm_after>>)
   .
 
   Hypothesis FINALFSIM: forall
@@ -253,11 +256,9 @@ Section MATCHSIMFORWARD.
         exploit AFTERFSIM; try apply SAFESRC; try apply SIMRET; eauto.
         { ii. eapply SUSTAR; eauto. eapply star_refl. apply tt. }
         { econs; eauto. }
-        { eapply SimMem.unlift_wf; eauto. }
-        { eapply SimMem.lift_spec; eauto. }
         i; des.
-        assert(MLE3: SimMem.le sm0 sm_after).
-        { etrans; cycle 1. { et. } etrans; et. eapply SimMem.lift_spec; et. }
+        assert(MLE4: SimMem.le sm0 sm_after).
+        { etrans; cycle 1. { et. } refl. }
         esplits; eauto.
         right.
         eapply CIH; eauto.
